refine+crefine: define and handle fastpathKernelAssertions
Currently, this is only interesting on AARCH64 where we need no_fail
preconditions for looking up an ASID map entry.

Signed-off-by: Rafal Kolanski <rafal.kolanski@proofcraft.systems>

proof/refine/ARM/PageTableDuplicates.thy
@@ -2234,13 +2234,17 @@ lemma handleEvent_valid_duplicates':
               | wpc)+
   done
 
+(* nothing extra needed on this architecture *)
+defs fastpathKernelAssertions_def:
+  "fastpathKernelAssertions \<equiv> \<lambda>s. True"
+
 lemma callKernel_valid_duplicates':
   "\<lbrace>invs' and (\<lambda>s. vs_valid_duplicates' (ksPSpace s)) and
     (\<lambda>s. ksSchedulerAction s = ResumeCurrentThread) and
     (\<lambda>s. e \<noteq> Interrupt \<longrightarrow> ct_running' s)\<rbrace>
    callKernel e
    \<lbrace>\<lambda>rv s. vs_valid_duplicates' (ksPSpace s)\<rbrace>"
-  apply (simp add: callKernel_def)
+  apply (simp add: callKernel_def fastpathKernelAssertions_def)
   apply (rule hoare_pre)
    apply (wp activate_invs' activate_sch_act schedule_sch
              schedule_sch_act_simple he_invs'
