proof/crefine/X64/Refine_C.thy
@@ -49,6 +49,7 @@ proof -
   show ?thesis
   apply (cinit')
    apply (simp add: callKernel_def handleEvent_def minus_one_norm)
+   apply (rule ccorres_stateAssert)
    apply (simp add: liftE_bind bind_assoc)
     apply (ctac (no_vcg) add: getActiveIRQ_ccorres)
     apply (rule ccorres_Guard_Seq)?
@@ -92,6 +93,7 @@ lemma handleUnknownSyscall_ccorres:
            (callKernel (UnknownSyscall n)) (Call handleUnknownSyscall_'proc)"
   apply (cinit' lift: w_')
    apply (simp add: callKernel_def handleEvent_def)
+   apply (rule ccorres_stateAssert)
    apply (simp add: liftE_bind bind_assoc)
    apply (rule ccorres_symb_exec_r)
      apply (rule ccorres_pre_getCurThread)
@@ -129,8 +131,10 @@ lemma handleVMFaultEvent_ccorres:
            (callKernel (VMFaultEvent vmfault_type)) (Call handleVMFaultEvent_'proc)"
   apply (cinit' lift:vm_faultType_')
    apply (simp add: callKernel_def handleEvent_def)
+   apply (rule ccorres_stateAssert)
    apply (simp add: liftE_bind bind_assoc)
    apply (rule ccorres_pre_getCurThread)
+   apply (rename_tac thread)
    apply (simp add: catch_def)
    apply (rule ccorres_rhs_assoc2)
    apply (rule ccorres_split_nothrow_novcg)
@@ -178,6 +182,7 @@ lemma handleUserLevelFault_ccorres:
            (callKernel (UserLevelFault word1 word2)) (Call handleUserLevelFault_'proc)"
   apply (cinit' lift:w_a_' w_b_')
    apply (simp add: callKernel_def handleEvent_def)
+   apply (rule ccorres_stateAssert)
    apply (simp add: liftE_bind bind_assoc)
    apply (rule ccorres_symb_exec_r)
      apply (rule ccorres_pre_getCurThread)
@@ -230,6 +235,7 @@ lemma handleSyscall_ccorres:
            (callKernel (SyscallEvent sysc)) (Call handleSyscall_'proc)"
   apply (cinit' lift: syscall_')
    apply (simp add: callKernel_def handleEvent_def minus_one_norm)
+   apply (rule ccorres_stateAssert)
    apply (simp add: handleE_def handleE'_def)
    apply (rule ccorres_split_nothrow_novcg)
        apply wpc
@@ -502,6 +508,7 @@ lemma handleHypervisorEvent_ccorres:
   apply (simp add: callKernel_def handleEvent_def handleHypervisorEvent_C_def)
   apply (simp add: liftE_def bind_assoc)
   apply (rule ccorres_guard_imp)
+    apply (rule ccorres_stateAssert)
     apply (rule ccorres_symb_exec_l)
        apply (cases t; simp add: handleHypervisorFault_def)
        apply (ctac (no_vcg) add: schedule_ccorres)
